Add repeat loop to the imperative language

smallstep_monad.v
@@ -20,10 +20,22 @@ Fixpoint denote {A : Type} (p : program A) : M A :=
   | p_ret _ v => Ret v
   | p_bind _ _ m f => do a <- denote m; denote (f a)
   | p_cond _ b p1 p2 => if b then denote p1 else denote p2
+  | p_repeat n p => (fix loop (m : nat) : M unit :=
+    match m with
+    | 0 => Ret tt
+    | Datatypes.S m' => denote p >> loop m'
+    end) n
   | p_get => stGet
   | p_put s' => stPut s'
   | p_mark t => stMark t
   end.
+
+Notation "'Repeat' n {{ p }}" := (
+  (fix loop (m : nat) : MonadStateTraceRun.m M unit :=
+   match m with
+   | 0 => Ret tt
+   | Datatypes.S m' => denote p >> loop m'
+   end) n) (at level 200).
 
 Fixpoint denote_continuation (k : continuation) : M (@continuation T S) :=
   match k with
@@ -46,7 +58,8 @@ Lemma denote_prefix_preserved A (m : M A) :
 Proof.
 intros [ p Hp ].
 subst m.
-induction p as [ A a | A B p IHp g IHg | A b p1 IHp1 p2 IHp2 | | s0 | t ]; cbn;
+induction p as [ A a | A B p IHp g IHg | A b p1 IHp1 p2 IHp2 |
+  n p IHp | | s0 | t ]; cbn;
  intros s s' l1 l a' Heq.
 - exists [].
   rewrite cats0.
@@ -63,6 +76,24 @@ induction p as [ A a | A B p IHp g IHg | A b p1 IHp1 p2 IHp2 | | s0 | t ]; cbn;
   rewrite catA.
   congruence.
 - destruct b; [ eapply IHp1 | eapply IHp2 ]; exact Heq.
+- revert s l1 Heq.
+  induction n as [ | n' IH ]; intros s l1 Heq.
+  + exists [].
+    rewrite cats0.
+    by move: Heq; rewrite runret => -[].
+  + rewrite runbind in Heq.
+    case_eq (Run (denote p) (s, l1)).
+    intros a (s0, l0) Hp.
+    specialize (IHp _ _ _ _ _ Hp).
+    destruct IHp as [l2 IHp ].
+    subst l0.
+    rewrite Hp in Heq.
+    specialize (IH _ _ Heq).
+    destruct IH as [l3 IH].
+    exists (l2 ++ l3).
+    subst l.
+    symmetry.
+    apply app_assoc.
 - exists [].
   rewrite cats0.
   by move: Heq; rewrite runstget => -[].
@@ -81,16 +112,26 @@ Lemma denote_prefix_independent A (m : M A) :
 Proof.
 intros [ p Hp ] s l1 l2.
 subst m.
-elim: p s l1 l2 => /= {A} [A a|A B p1 IH1 p2 IH2|A b p1 IH1 p2 IH2||s'|t] s l1 l2.
-by rewrite !runret.
-rewrite [in LHS]runbind [in LHS]IH1.
+elim: p s l1 l2 => /= {A} [A a|A B p1 IH1 p2 IH2|A b p1 IH1 p2 IH2|
+  n p IHp||s'|t] s l1 l2.
+- by rewrite !runret.
+- rewrite [in LHS]runbind [in LHS]IH1.
 rewrite [in RHS]runbind.
 case: (Run (denote p1) (s, l2)) => a' [s' l'] /=.
 by rewrite IH2.
-by case: ifPn => _; [rewrite IH1|rewrite IH2].
-by rewrite !runstget.
-by rewrite !runstput.
-by rewrite !runstmark rcons_cat.
+- by case: ifPn => _; [rewrite IH1|rewrite IH2].
+- revert s l2.
+  induction n as [ | n' IH ]; intros s l2.
+  + by rewrite !runret.
+  + do 2 rewrite runbind.
+    rewrite IHp.
+    clear IHp.
+    case_eq (Run (denote p) (s, l2)).
+    intros a (s0, l0) Hp.
+    apply IH.
+- by rewrite !runstget.
+- by rewrite !runstput.
+- by rewrite !runstmark rcons_cat.
 Qed.
 
 Lemma denote_continuation_prefix_independent m :
@@ -119,7 +160,8 @@ remember None as o eqn: Heqo.
 remember (s', k') as sk' eqn: Heq'.
 revert s s' k k' l Heq Heq' Heqo.
 induction Hstep as
- [ s A a f | s A B p f g | s A p1 p2 k | s A p1 p2 k | s f | s s' f | s t f ];
+ [ s A a f | s A B p f g | s A p1 p2 k | s A p1 p2 k |
+   s p k | s n p k | s f | s s' f | s t f ];
  intros s1 s2 k1 k2 l [= Hs1 Hk1] [= Hs2 Hk2] Heqo.
 - subst s1 k1 s2 k2.
   by rewrite /= runbind runret.
@@ -129,6 +171,14 @@ induction Hstep as
 - subst s1 s2 k1 k2.
   reflexivity.
 - subst s1 s2 k1 k2.
+  reflexivity.
+- subst.
+  cbn.
+  rewrite bindretf.
+  reflexivity.
+- subst.
+  cbn.
+  rewrite bindA.
   reflexivity.
 - subst s1 k1 s2 k2.
   by rewrite /= runbind runstget.
@@ -148,7 +198,8 @@ remember (Some t) as o eqn: Heqo.
 remember (s', k') as sk' eqn: Heq'.
 revert s s' k k' l Heq Heq' Heqo.
 induction Hstep as
- [ s A a f | s A B p f g | s A p1 p2 k | s A p1 p2 k | s f | s s' f | s t' f ];
+ [ s A a f | s A B p f g | s A p1 p2 k | s A p1 p2 k |
+   s p k | s n p k | s f | s s' f | s t' f ];
  intros s1 s2 k1 k2 l [= Hs1 Hk1] [= Hs2 Hk2] Heqo; try discriminate Heqo.
 subst s1 k1 s2 k2.
 injection Heqo; intro; subst t.
@@ -210,7 +261,8 @@ Lemma step_star_complete_gen
   step_star (s, p `; f) l2 (s', f a).
 Proof.
 revert s s' a l1 l2 f.
-induction p as [ A a | A B p IHp g IHg | A b p1 IHp1 p2 IHp2 | |  aa | t ]; cbn;
+induction p as [ A a | A B p IHp g IHg | A b p1 IHp1 p2 IHp2 |
+  n p IH | | s0' | t ]; cbn;
  intros s s' a' l1 l2 f Heq.
 - rewrite runret in Heq.
   injection Heq; clear Heq; intros; subst a' s'.
@@ -247,6 +299,41 @@ induction p as [ A a | A B p IHp g IHg | A b p1 IHp1 p2 IHp2 | |  aa | t ]; cbn;
       apply s_cond_false
     | apply IHp2 with (l1 := l1); exact Heq ]
   ].
+- revert s l1 l2 Heq.
+  induction n as [ | n' IHn ]; intros s l1 l2 Heq.
+  + rewrite runret in Heq.
+    injection Heq; clear Heq; intros; subst a' s'.
+    replace l2 with (@nil T) by
+     (revert l2 H; induction l1; [ tauto | intros ? [=]; firstorder ]).
+    eapply ss_step_None; [ apply s_repeat_O | apply ss_refl ].
+  + rewrite runbind in Heq.
+    case_eq (Run (denote p) (s, l1)).
+    intros a (s0, l0) Hp.
+    rewrite Hp in Heq.
+    specialize (denote_prefix_preserved _ _ ltac:(now eexists) _ _ _ _ _ Hp).
+    intros [l3 Hl3].
+    rewrite Hl3 in Hp, Heq.
+    clear l0 Hl3.
+    specialize (IH _ _ _ _ _ (fun _ => p_repeat n' p `; f) Hp).
+    assert (Heq':
+     Run (denote (p_repeat n' p)) (s0, l1 ++ l3) = (a', (s', l1 ++ l2)))
+     by apply Heq.
+    specialize (denote_prefix_preserved _ _ ltac:(now eexists) _ _ _ _ _ Heq').
+    intros [l4 Hl4].
+    rewrite Hl4 in Heq.
+    eapply ss_step_None; [ apply s_repeat_S | ].
+    assert (Hl2: l2 = l3 ++ l4).
+    {
+      revert Hl4.
+      clear.
+      induction l1 as [ | a1 l1 IH ]; [ trivial | ].
+      cbn.
+      intro H.
+      apply IH.
+      injection H; trivial.
+    }
+    rewrite Hl2.
+    eapply step_star_transitive; [ eexact IH | eapply IHn; eexact Heq ].
 - rewrite runstget in Heq.
   injection Heq; clear Heq; intros; subst a' s'.
   replace l2 with (@nil T) by
